Successfully verified correctness of filter count

Dafny/Searching.dfy
@@ -1,18 +1,67 @@
-// Assuming Array is Object Blood.
-// Blood Array<int> 
-// index 
+/* Filtering
+ * Lucas and Rason
+ *
+ * Currently filters an array of integers given a specified test.
+ * Can later extend to filter blood objects by blood type.
+ */
 
-method Find(blood: array<int>, key: int) returns (index: int)
-   ensures 0 <= index ==> index < blood.Length && blood[index] == key
-   ensures index < 0 ==> forall k :: 0 <= k < blood.Length ==> blood[k] != key
+// Some sample tests with integers
+predicate method testEven(x: int) { x % 2 == 0 }
+predicate method testPositive(x: int) { x > 0 }
+// (must be function methods for some reason, does anyone know why?)
+
+method Main()
 {
-   index := 0;
-   while index < blood.Length
-      invariant 0 <= index <= blood.Length
-      invariant forall k :: 0 <= k < index ==> blood[k] != key
-   {
-      if blood[index] == key { return; }
-      index := index + 1;
-   }
-   index := -1;
+  var a := new int[10];
+  a[0], a[1], a[2], a[3], a[4], a[5], a[6], a[7], a[8], a[9] := -1, 2, -5, -4, 1, -2, -3, 3, 0, 4;
+  print "original: ", a[..], "\n";
+
+  var b := Filter(a, testEven);
+  print "even    : ", b[..], "\n"; assert b.Length == 5;
+
+  b := Filter(a, testPositive);
+  print "positive: ", b[..], "\n"; assert b.Length == 4;
+}
+
+// Returns a new array containing only those elements that pass a specified test
+method Filter(a: array<int>, test: int -> bool) returns (b: array<int>)
+requires a != null
+requires forall i :: test.requires(i) && |test.reads(i)| == 0
+ensures b != null
+ensures b.Length == Matches(a, a.Length, test);
+{
+  var matches := 0;
+  var i := 0;
+  while i < a.Length
+  invariant 0 <= i <= a.Length && matches == Matches(a, i, test)
+  {
+    if test(a[i]) { matches := matches + 1; }
+    i := i + 1;
+  }
+  b := new int[matches];
+
+  // TODO: still thinking about how to properly verify below
+  i := 0;
+  var j := 0;
+  while i < a.Length && j < matches
+  {
+    if test(a[i])
+    {
+      b[j] := a[i];
+      j := j + 1;
+    }
+    i := i + 1;
+  }
+}
+
+// Verifies the number of matches given a specified array and test function.
+function Matches(a: array<int>, top: nat, test: int -> bool): int
+reads a
+requires a != null
+requires top <= a.Length
+requires forall i :: test.requires(i) && |test.reads(i)| == 0
+decreases top // (fails asserts without this, does anyone know why?)
+{
+  if top < 1 then 0 else
+    (if test(a[top-1]) then 1 else 0) + Matches(a, top-1, test)
 }
